Indexing stuff is "done", but at what cost?

Hashmap/DHashMap/Basic.lean
@@ -6,6 +6,7 @@ Authors: Leonardo de Moura, Mario Carneiro, Markus Himmel
 import Hashmap.AssocList.Basic
 import Hashmap.LawfulHashable
 import Std.Data.Array.Lemmas
+import Hashmap.DHashMap.Index
 
 set_option autoImplicit false
 
@@ -34,28 +35,24 @@ def empty (capacity := 8) : Raw α β where
   size := 0
   buckets := mkArray (numBucketsForCapacity capacity).nextPowerOfTwo AssocList.nil
 
-def mkIdx {sz : Nat} (hash : UInt64) (h : 0 < sz) : { u : USize // u.toNat < sz } :=
-  -- TODO: restore this to hash.toUSize &&& (sz.toUSize - 1). This is not so easy because we probably (?) don't want
-  -- to check for m.buckets.size.isPowerOfTwo in Raw.insert, right?
-  ⟨hash.toUSize % sz, Nat.mod_lt _ h⟩
 
 @[inline] def reinsertAux [Hashable α]
-    (data : { d : Array (AssocList α β) // 0 < d.size }) (a : α) (b : β a) : { d : Array (AssocList α β) // 0 < d.size } :=
+    (data : { d : Array (AssocList α β) // IsGoodSize d.size }) (a : α) (b : β a) : { d : Array (AssocList α β) // IsGoodSize d.size } :=
   let ⟨data, hd⟩ := data
   let ⟨i, h⟩ := mkIdx (hash a) hd
   ⟨data.uset i (data[i].cons a b) h, by simpa⟩
 
 /-- Copies all the entries from `buckets` into a new hash map with a larger capacity. -/
-def expand [Hashable α] (size : Nat) (data : { d : Array (AssocList α β) // 0 < d.size }) : { m : Raw α β // 0 < m.buckets.size } :=
+def expand [Hashable α] (size : Nat) (data : { d : Array (AssocList α β) // IsGoodSize d.size }) : { m : Raw α β // IsGoodSize m.buckets.size } :=
   let ⟨data, hd⟩ := data
-  let nbuckets := data.size * 2
-  let ⟨newBuckets, hn⟩ := go 0 data ⟨mkArray nbuckets AssocList.nil, by rw [Array.size_mkArray]; exact Nat.mul_pos hd Nat.two_pos⟩
+  let ⟨nbuckets, hnbuckets⟩ := nextSize ⟨_, hd⟩
+  let ⟨newBuckets, hn⟩ := go 0 data ⟨mkArray nbuckets AssocList.nil, by simpa⟩
   ⟨{ size, buckets := newBuckets }, hn⟩
 where
   /-- Inner loop of `expand`. Copies elements `source[i:]` into `target`,
   destroying `source` in the process. -/
-  go (i : Nat) (source : Array (AssocList α β)) (target : { d : Array (AssocList α β) // 0 < d.size }) :
-      { d : Array (AssocList α β) // 0 < d.size } :=
+  go (i : Nat) (source : Array (AssocList α β)) (target : { d : Array (AssocList α β) // IsGoodSize d.size }) :
+      { d : Array (AssocList α β) // IsGoodSize d.size } :=
     if h : i < source.size then
       let idx : Fin source.size := ⟨i, h⟩
       let es := source.get idx
@@ -67,8 +64,8 @@ where
     else target
   termination_by source.size - i
 
-@[inline] def insertWellFormed [BEq α] [Hashable α] (m : { m : Raw α β // 0 < m.buckets.size }) (a : α) (b : β a) :
-    { m : Raw α β // 0 < m.buckets.size } × Bool :=
+@[inline] def insertWellFormed [BEq α] [Hashable α] (m : { m : Raw α β // IsGoodSize m.buckets.size }) (a : α) (b : β a) :
+    { m : Raw α β // IsGoodSize m.buckets.size } × Bool :=
   let ⟨⟨size, buckets⟩, hm⟩ := m
   let ⟨i, h⟩ := mkIdx (hash a) hm
   let bkt := buckets[i]
@@ -83,23 +80,23 @@ where
       (expand size' ⟨buckets', by simpa [buckets']⟩, false)
 
 @[inline] def insert' [BEq α] [Hashable α] (m : Raw α β) (a : α) (b : β a) : Raw α β × Bool :=
-  if h : 0 < m.buckets.size then
-    let ⟨⟨r, _⟩, replaced⟩ := insertWellFormed ⟨m, h⟩ a b
+  if h : checkSize m.buckets.size = true then
+    let ⟨⟨r, _⟩, replaced⟩ := insertWellFormed ⟨m, checkSize_eq_true.1 h⟩ a b
     ⟨r, replaced⟩
   else (m, false) -- will never happen for well-formed inputs
 
 @[inline] def insert [BEq α] [Hashable α] (m : Raw α β) (a : α) (b : β a) : Raw α β :=
   (insert' m a b).1
 
-@[inline] def findEntry?WellFormed [BEq α] [Hashable α] (m : { m : Raw α β // 0 < m.buckets.size }) (a : α) :
+@[inline] def findEntry?WellFormed [BEq α] [Hashable α] (m : { m : Raw α β // IsGoodSize m.buckets.size }) (a : α) :
     Option (Σ a, β a) :=
   let ⟨⟨_, buckets⟩, h⟩ := m
   let ⟨i, h⟩ := mkIdx (hash a) h
   buckets[i].findEntry? a
 
 @[inline] def findEntry? [BEq α] [Hashable α] (m : Raw α β) (a : α) : Option (Σ a, β a) :=
-  if h : 0 < m.buckets.size then
-    findEntry?WellFormed ⟨m, h⟩ a
+  if h : checkSize m.buckets.size = true then
+    findEntry?WellFormed ⟨m, checkSize_eq_true.1 h⟩ a
   else none -- will never happen for well-formed inputs
 
 section WF
@@ -107,38 +104,50 @@ section WF
 def toList (m : Raw α β) : List (Σ a, β a) :=
   m.buckets.data.bind AssocList.toList
 
-structure WF [BEq α] [Hashable α] (m : Raw α β) : Prop where
+structure ActuallyWF [BEq α] [Hashable α] (m : Raw α β) : Prop where
   buckets_hash_self : IsHashSelf m.buckets
-  buckets_size : m.buckets.size.isPowerOfTwo
+  buckets_size : IsGoodSize m.buckets.size
   size_eq : m.size = m.toList.length
   distinct : m.toList.WF
+
+inductive WF [BEq α] [Hashable α] : Raw α β → Prop where
+  | wf : ∀ m, m.ActuallyWF → WF m
+  | insertWellFormed : ∀ m h a b, WF m → WF (Raw.insertWellFormed ⟨m, h⟩ a b).1.1
+
+theorem WF.size_buckets_pos [BEq α] [Hashable α] (m : Raw α β) : WF m → IsGoodSize m.buckets.size
+  | wf m h => h.buckets_size
+  | insertWellFormed m h a b _ => (Raw.insertWellFormed ⟨m, h⟩ a b).1.2
+
+theorem WF.insert' [BEq α] [Hashable α] {m : Raw α β} {a : α} {b : β a} (h : m.WF) : (m.insert' a b).1.WF := by
+  rw [Raw.insert']
+  split
+  · next h' => exact .insertWellFormed _ (checkSize_eq_true.1 h') _ _ h
+  · exact h
+
+theorem WF.insert [BEq α] [Hashable α] {m : Raw α β} {a : α} {b : β a} (h : m.WF) : (m.insert a b).WF :=
+  WF.insert' h
 
 end WF
 
 end Raw
 
-inductive WF [BEq α] [Hashable α] : Raw α β → Prop where
-  | wf : ∀ m, m.WF → WF m
-  | insert : ∀ m h a b, WF (Raw.insertWellFormed ⟨m, h⟩ a b).1.1
-
-theorem WF.size_buckets_pos [BEq α] [Hashable α] (m : Raw α β) : WF m → 0 < m.buckets.size
-  | wf m h => Nat.pos_of_isPowerOfTwo h.buckets_size
-  | insert m h a b => (Raw.insertWellFormed ⟨m, h⟩ a b).1.2
 
 end DHashMap
 
-def DHashMap (α : Type u) (β : α → Type v) [BEq α] [Hashable α] := { m : DHashMap.Raw α β // DHashMap.WF m }
+def DHashMap (α : Type u) (β : α → Type v) [BEq α] [Hashable α] := { m : DHashMap.Raw α β // m.WF }
 
 namespace DHashMap
 
 @[inline] def insert' [BEq α] [Hashable α] (m : DHashMap α β) (a : α) (b : β a) : DHashMap α β × Bool :=
   let m' := Raw.insertWellFormed ⟨m.1, m.2.size_buckets_pos⟩ a b
-  ⟨⟨m'.1.1, .insert _ _ _ _⟩, m'.2⟩
+  ⟨⟨m'.1.1, .insertWellFormed _ _ _ _ m.2⟩, m'.2⟩
 
 @[inline] def insert [BEq α] [Hashable α] (m : DHashMap α β) (a : α) (b : β a) : DHashMap α β :=
   (m.insert' a b).1
 
 @[inline] def findEntry? [BEq α] [Hashable α] (m : DHashMap α β) (a : α) : Option (Σ a, β a) :=
   Raw.findEntry?WellFormed ⟨m.1, m.2.size_buckets_pos⟩ a
+
+#eval ((Raw.empty : Raw Nat (fun _ => Nat)).insert 2 3).findEntry? 2
 
 end MyLean.DHashMap
